\documentclass{article}
\usepackage{mathtools}
\begin{document}


% F_y by limit definition
\begin{align*}
f_y &= \lim_{h\to\infty} \frac{f(a, b+h) - f(a,b)}{h} \\
&= \lim_{h\to\infty} (\frac{1}{h}) (\frac{a^3(b+h) - a(b+h)^3}{a^2+(b+h)^2} - \frac{a^3b-ab^3}{a^2+b^2}) \\
&= \lim_{h\to\infty} (\frac{1}{h}) (\frac{a^3(b+h) - a(b+h)(b+h)(b+h)}{a^2+(b+h)(b+h)} - \frac{a^3b-ab^3}{a^2+b^2}) \\
&= \lim_{h\to\infty} (\frac{1}{h}) (\frac{a^3(b+h) - a(b^3+3b^2h+3bh^2+h^3)}{a^2+b^2+2bh+h^2} - \frac{a^3b-ab^3}{a^2+b^2}) \\
&= \lim_{h\to\infty} (\frac{1}{h}) (\frac{a^3b+a^3h-ab^3-3ab^2h-3abh^2-ah^3}{a^2+b^2+2bh+h^2} - \frac{a^3b-ab^3}{a^2+b^2}) \\
&= \lim_{h\to\infty} (\frac{1}{h}) (\frac{(a^2+b^2)(a^3b+a^3h-ab^3-3ab^2h-3abh^2-ah^3)}{a^2+b^2+2bh+h^2} - \frac{(a^2+b^2+bh+h^2)(a^3b-ab^3)}{a^2+b^2}) \\
&= \lim_{h\to\infty} (\frac{1}{h}) (\frac{a^5b+a^5h-a^3b^3-3a^3b^2h-3a^3bh^2-a^3h^3+a^3b^3+a^3b^2h-ab^5+3ab^4h+3ab^3h^2+ab^2h^3-(a^5b-a^3b^3+a^3b^3-ab^5+2a^3b^2h-2ab^4h+a^3bh^2-ab^3h^2)}{a^4+a^2b^2+2a^bh+a^2h^2+a^2b^2+2b^2h+b^2h^2+b^4}) \\
&= \lim_{h\to\infty} (\frac{1}{h}) (\frac{a^5h-3a^3b^2h-3a^3bh^2-a^3h^3+a^3b^2h-3ab^4h+3ab^3h^2+ab^2h^3-2a^3b^2h+2ab^4h-a^3bh^2+ab^3h^2}{a^4+a^2b^2+2a^bh+a^2h^2+a^2b^2+2b^2h+b^2h^2+b^4}) \\
&= \lim_{h\to\infty} (\frac{1}{h}) (\frac{a^5h-4a^3b^2h-4a^3bh^2+4ab^3h^2-ab^4h+ab^2h^3}{a^4+a^2b^2+2a^bh+a^2h^2+a^2b^2+2b^2h+b^2h^2+b^4}) \\
&= \lim_{h\to\infty} (\frac{1}{h}) (\frac{a^5-4a^3bh+4ab^3h-ab^4+ab^2h-4a^3b^2h}{a^4+a^2b^2+2a^bh+a^2h^2+a^2b^2+2b^2h+b^2h^2+b^4}) \\
&= \frac{a^5-4a^3b^2-ab^4}{a^4+2a^2b^2} \\
&= \frac{a(a^4-4a^2b^2-ab^4)}{a^4+2a^2b^2} \\
\end{align*}
Set a = 0
\begin{align*}
& \lim_{b\to0} \frac{0(0^4-4(0^3)b^2-(0)b^4)}{0^4+2(0^2)b^2+b^4} \\
\lim_{b\to0} & \frac{0}{b^4} &&= \frac{0}{0} \\
\lim_{b\to0} & \frac{0}{4b^3} &&= \frac{0}{0} \\
\lim_{b\to0} & \frac{0}{12b^2} &&= \frac{0}{0} \\
\lim_{b\to0} & \frac{0}{24b} &&= \frac{0}{0} \\
\lim_{b\to0} & \frac{0}{24} &&= 0 \\
\end{align*}

% end F_y by limit definition

\end{document}